verify/Flip.v
@@ -1,0 +1,125 @@
+(** * Flip: swapping left and right *)
+
+Set Warnings "-notation-overriden,-parsing,-deprecated-hint-without-locality".
+From Coq Require Import Logic.FunctionalExtensionality.
+From Coq Require Import Bool.
+From Coq Require Import Lists.List. Import ListNotations.
+From Coq Require Import Lia.
+From BusyCoq Require Export Compute.
+Set Default Goal Selector "!".
+
+Module Flip (Ctx : Ctx).
+  Local Module Compute := Compute Ctx. Export Compute.
+
+Definition flip_dir (d : dir) :=
+  match d with
+  | L => R
+  | R => L
+  end.
+
+Definition flip_tape (t : tape) :=
+  match t with
+  | l {{s}} r => r {{s}} l
+  end.
+
+Lemma flip_move_left : forall t,
+  flip_tape (move_left t) = move_right (flip_tape t).
+Proof.
+  intros [[[u l] s] r]. reflexivity.
+Qed.
+
+Lemma flip_move_right : forall t,
+  flip_tape (move_right t) = move_left (flip_tape t).
+Proof.
+  intros [[l s] [u r]]. reflexivity.
+Qed.
+
+Arguments move_left : simpl never.
+Arguments move_right : simpl never.
+
+Definition flip (tm : TM) : TM := fun qs =>
+  match tm qs with
+  | Some (s, d, q) => Some (s, flip_dir d, q)
+  | None => None
+  end.
+
+Lemma flip_involutive : forall tm,
+  flip (flip tm) = tm.
+Proof.
+  intros tm. apply functional_extensionality.
+  intros [q s]. unfold flip.
+  destruct (tm (q, s)) as [[[s' []] q'] |]; reflexivity.
+Qed.
+
+Definition flip_conf (c : Q * tape) : Q * tape :=
+  match c with
+  | q; t => q; flip_tape t
+  end.
+
+Lemma flip_conf_involutive : forall c,
+  flip_conf (flip_conf c) = c.
+Proof.
+  intros [q [[l s] r]]. reflexivity.
+Qed.
+
+Lemma flip_step : forall tm c c',
+  c -[ tm ]-> c' ->
+  flip_conf c -[ flip tm ]-> flip_conf c'.
+Proof.
+  introv H.
+  inverts H as E.
+  - simpl. rewrite flip_move_left. apply step_right.
+    unfold flip. rewrite E. reflexivity.
+  - simpl. rewrite flip_move_right. apply step_left.
+    unfold flip. rewrite E. reflexivity.
+Qed.
+
+Lemma flip_multistep : forall tm n c c',
+  c -[ tm ]->* n / c' ->
+  flip_conf c -[ flip tm ]->* n / flip_conf c'.
+Proof.
+  induction n; introv H; inverts H as Hstep Hrest.
+  - apply multistep_0.
+  - eauto using flip_step, multistep_S.
+Qed.
+
+Lemma flip_halting : forall tm c,
+  halting tm c -> halting (flip tm) (flip_conf c).
+Proof.
+  intros tm [q [[l s] r]].
+  unfold halting, flip. simpl.
+  intros H. rewrite H.
+  reflexivity.
+Qed.
+
+Lemma flip_halts_in : forall tm c n,
+  halts_in tm c n -> halts_in (flip tm) (flip_conf c) n.
+Proof.
+  introv H.
+  destruct H as [ch [Hexec Hhalting]].
+  apply flip_multistep in Hexec.
+  apply flip_halting in Hhalting.
+  eexists. split; eassumption.
+Qed.
+
+Lemma flip_halts : forall tm c,
+  halts tm c -> halts (flip tm) (flip_conf c).
+Proof.
+  introv H. destruct H as [n H].
+  exists n. apply flip_halts_in. assumption.
+Qed.
+
+Lemma flip_halts_iff : forall tm c,
+  halts tm c <-> halts (flip tm) (flip_conf c).
+Proof.
+  introv. split.
+  - apply flip_halts.
+  - intros H. apply flip_halts in H.
+    rewrite flip_involutive, flip_conf_involutive in H.
+    exact H.
+Qed.
+
+Lemma flip_c0 : flip_conf c0 = c0.
+Proof. reflexivity. Qed.
+
+End Flip.
